aneris/aneris_lang/program_logic/atomic.v
@@ -1,6 +1,6 @@
 From stdpp Require Import namespaces.
 From iris.bi Require Import telescopes.
-From iris.bi.lib Require Export atomic.
+From iris.bi.lib Require Export atomic laterable.
 From iris.proofmode Require Import tactics classes.
 From aneris.aneris_lang.program_logic Require Export aneris_weakestpre.
 From iris.base_logic Require Import invariants.
