aneris/examples/reliable_communication/lib/repdb/proof/proof_of_db_init.v
@@ -122,7 +122,7 @@ Section Init_setup_proof.
     iDestruct (big_sepM_delete _ N DB_addrF γdbF with "Htks")
       as "#(HtkF & Htks')"; first done.
     set (initL := init_leader_res γL γM N SrvInit SrvInitF γdbF).
-    rewrite -{4} Qp_half_half.
+    rewrite -{4} Qp.half_half.
     iDestruct (own_log_auth_split _ (1/2) (1/2) [] with "[$HlogLM]")
       as "(HlogL1 & HlogL2)".
     iMod (inv_alloc
